src/partie2.v
@@ -2,15 +2,15 @@ Add LoadPath "." as CoqDirectory.
 Load partie1.
 
 Inductive beta_reduction_one_step : DeBruijn -> DeBruijn -> Prop :=
-    | Evaluation : forall (u: DeBruijn), forall (v: DeBruijn), 
+    | Evaluation : forall (u v: DeBruijn),
         (beta_reduction_one_step (Application (Lambda u) v) (u[0 <- v]))
-    | Context_r : forall (u: DeBruijn), forall (v: DeBruijn), forall (w: DeBruijn),
+    | Context_r : forall (u v w: DeBruijn),
         (beta_reduction_one_step v w) -> 
             (beta_reduction_one_step (Application u v) (Application u w))
-    | Context_l : forall (u: DeBruijn), forall (v: DeBruijn), forall (w: DeBruijn),
+    | Context_l : forall (u v w: DeBruijn),
         (beta_reduction_one_step u v) -> 
             (beta_reduction_one_step (Application u w) (Application v w))
-    | Context_lambda : forall (u: DeBruijn), forall (v: DeBruijn),
+    | Context_lambda : forall (u v: DeBruijn),
         (beta_reduction_one_step u v) -> (beta_reduction_one_step (Lambda u) (Lambda v)) 
 .
 
@@ -18,7 +18,7 @@ Inductive beta_reduction_one_step : DeBruijn -> DeBruijn -> Prop :=
 
 Inductive beta_reduction : DeBruijn -> DeBruijn -> Prop :=
     | beta_refl : forall (u: DeBruijn), beta_reduction u u
-    | beta_trans : forall (t: DeBruijn), forall (u: DeBruijn), forall (v: DeBruijn),
+    | beta_trans : forall (t u v: DeBruijn),
         (beta_reduction_one_step t u) -> (beta_reduction u v) -> (beta_reduction t v)
 .
 
@@ -32,7 +32,7 @@ destruct H.
     apply Context_l. exact H.
 *)
 
-Theorem context_l_star : forall (t:DeBruijn), forall (u: DeBruijn), forall (v: DeBruijn),
+Theorem context_l_star : forall (t u v: DeBruijn),
     t -b>* u -> (Application t v) -b>* (Application u v).
 Proof.
     move => t u v.
@@ -44,7 +44,7 @@ Proof.
     apply (beta_trans (Application t v) (Application u v) (Application v0 v) H1 IHbeta_reduction).
 Qed.
 
-Theorem context_r_star : forall (t:DeBruijn), forall (u: DeBruijn), forall (v: DeBruijn),
+Theorem context_r_star : forall (t u v: DeBruijn),
     u -b>* v -> (Application t u) -b>* (Application t v).
 Proof.
     move => t u v.
@@ -56,7 +56,7 @@ Proof.
     apply (beta_trans (Application t t0) (Application t u) (Application t v) H1 IHbeta_reduction).
 Qed.
 
-Theorem context_lambda_star : forall (t: DeBruijn), forall (u: DeBruijn),
+Theorem context_lambda_star : forall (t u: DeBruijn),
     t -b>* u -> (Lambda t) -b>* (Lambda u).
 Proof.
     move => t u.
